theories/examples/bit.v
@@ -1,7 +1,6 @@
 From iris.proofmode Require Import tactics.
 From reloc Require Import reloc.
-From reloc.typing Require Import types interp fundamental.
-From reloc.typing Require Import soundness.
+Set Default Proof Using "Type".
 
 (* TODO: these modules should be values -- but we don't have refines_pair for values *)
 Definition bit_bool : expr :=
@@ -60,28 +59,6 @@ End bit_refinement.
 Theorem bit_ctx_refinement :
   ∅ ⊨ bit_bool ≤ctx≤ bit_nat : bitτ.
 Proof.
-  eapply (logrel_ctxequiv relocΣ).
-  iIntros (? ? vs) "Hvs". simpl.
-  (* TODO: this is not the place to have this boilerplate *)
-  rewrite !lookup_delete.
-  iApply (bit_refinement Δ).
+  eapply (refines_sound relocΣ).
+  iIntros (? Δ). iApply (bit_refinement Δ).
 Qed.
-
-(* Definition heapify : val := λ: "b", Unpack "b" $ λ: "b'", *)
-(*   let: "init" := Fst (Fst "b'") in *)
-(*   let: "flip" := Snd (Fst "b'") in *)
-(*   let: "view" := Snd "b'" in *)
-(*   let: "x" := ref "init" in *)
-(*   let: "l" := newlock #() in *)
-(*   let: "flip_ref" := λ: <>, acquire "l";; "x" <- "flip" (!"x");; release "l" in *)
-(*   let: "view_ref" := λ: <>, "view" (!"x") in *)
-(*   (#(), "flip_ref", "view_ref"). *)
-
-(* Lemma heapify_type Γ : *)
-(*   typed Γ heapify (TArrow bitτ bitτ). *)
-(* Proof. *)
-(*   unfold bitτ. unfold heapify. *)
-(*   unlock. *)
-(*   repeat (econstructor; solve_typed). (* TODO: solve_typed does not work by itself :( *) *)
-(* Qed. *)
-(* Hint Resolve heapify_type : typeable. *)
