theories/lib/assert.v
@@ -1,7 +1,5 @@
-From iris.heap_lang Require Export lang.
-From iris.proofmode Require Import tactics.
-From iris.heap_lang.lib Require Export assert.
 From reloc Require Import reloc.
+From iris.heap_lang.lib Require Export assert.
 Set Default Proof Using "Type".
 
 Definition assert : val :=
